src/Prog.v
@@ -1,6 +1,7 @@
 Require Import Arith.
 Require Import Word.
 Require Import FunctionalExtensionality.
+Require Import Eqdep.
 
 Set Implicit Arguments.
 
@@ -31,105 +32,100 @@ Definition wringaddr := wring addrlen.
 Add Ring wringaddr : wringaddr (decidable (weqb_sound addrlen), constants [wcst]).
 
 Inductive prog : Set -> Type :=
-| Done (t: donetoken)
-| Read (a: addr) (rx: valu -> prog)
-| Write (a: addr) (v: valu) (rx: unit -> prog).
+| Return {R: Set} (v: R) : prog R
+| Read (a: addr) : prog valu
+| Write (a: addr) (v: valu) : prog unit
+| Seq {T R: Set} (p1: prog T) (p2: T -> prog R) : prog R.
 
-Definition progseq (A B:Type) (a:B->A) (b:B) := a b.
-
-Notation "p1 ;; p2" := (progseq p1 (fun _: unit => p2)) (at level 60, right associativity).
-Notation "x <- p1 ; p2" := (progseq p1 (fun x => p2)) (at level 60, right associativity).
+Notation "p1 ;; p2" := (Seq p1 (fun _: unit => p2)) (at level 60, right associativity).
+Notation "x <- p1 ; p2" := (Seq p1 (fun x => p2)) (at level 60, right associativity).
 
 
 Definition mem := addr -> option valu.
 Definition upd (m : mem) (a : addr) (v : valu) : mem :=
   fun a' => if addr_eq_dec a' a then Some v else m a'.
 
-Inductive outcome :=
+Inductive outcome {R: Set} :=
 | Failed
-| Finished
-| Crashed.
+| Crashed (m: mem)
+| Finished (v: R) (m: mem).
 
-Inductive exec : mem -> prog -> mem -> outcome -> Prop :=
-| XDone : forall m t, exec m (Done t) m Finished
-| XReadFail : forall m a rx,
-  m a = None ->
-  exec m (Read a rx) m Failed
-| XWriteFail : forall m a v rx,
-  m a = None ->
-  exec m (Write a v rx) m Failed
-| XReadOK : forall m a v rx m' out,
-  m a = Some v ->
-  exec m (rx v) m' out ->
-  exec m (Read a rx) m' out
-| XWriteOK : forall m a v v0 rx m' out,
-  m a = Some v0 ->
-  exec (upd m a v) (rx tt) m' out ->
-  exec m (Write a v rx) m' out
-| XCrash : forall m p, exec m p m Crashed.
+Inductive exec : forall (R: Set), mem -> prog R -> @outcome R -> Prop :=
+| XReturn : forall m R v, exec m (@Return R v) (Finished v m)
+| XReadFail : forall m a, m a = None
+  -> exec m (Read a) Failed
+| XWriteFail : forall m a v, m a = None
+  -> exec m (Write a v) Failed
+| XReadOK : forall m a v, m a = Some v
+  -> exec m (Read a) (Finished v m)
+| XWriteOK : forall m a v v0, m a = Some v0
+  -> exec m (Write a v) (Finished tt (upd m a v))
+| XSeqFail : forall R T m p1 p2, exec m p1 (@Failed R)
+  -> exec m (Seq p1 p2) (@Failed T)
+| XSeqCrash : forall R T m p1 p2 m', exec m p1 (@Crashed R m')
+  -> exec m (Seq p1 p2) (@Crashed T m')
+| XSeqOK : forall R T m p1 p2 v m' (out: @outcome T), exec m p1 (@Finished R v m')
+  -> exec m' (p2 v) out
+  -> exec m (Seq p1 p2) out
+| XCrashBefore : forall R m p, exec m p (@Crashed R m)
+| XCrashAfter : forall R m p v m', exec m p (@Finished R v m')
+  -> exec m p (@Crashed R m').
 
-Inductive exec_recover : mem -> prog -> prog -> mem -> outcome -> Prop :=
-| XRFail : forall m p1 p2 m',
-  exec m p1 m' Failed -> exec_recover m p1 p2 m' Failed
-| XRFinished : forall m p1 p2 m',
-  exec m p1 m' Finished -> exec_recover m p1 p2 m' Finished
-| XRCrashed : forall m p1 p2 m' m'' out,
-  exec m p1 m' Crashed ->
-  exec_recover m' p2 p2 m'' out -> exec_recover m p1 p2 m'' out.
+Inductive exec_recover : forall (R: Set), mem -> prog R -> prog unit -> @outcome R -> Prop :=
+| XRFail : forall R m p1 p2, exec m p1 (@Failed R)
+  -> exec_recover m p1 p2 Failed
+| XRFinished : forall R m p1 p2 v m', exec m p1 (@Finished R v m')
+  -> exec_recover m p1 p2 (Finished v m')
+| XRCrashFail : forall R m p1 p2 m', exec m p1 (@Crashed R m')
+  -> exec_recover m' p2 p2 Failed
+  -> exec_recover m p1 p2 Failed
+| XRCrashFinished : forall R m p1 p2 m' v m'', exec m p1 (@Crashed R m')
+  -> exec_recover m' p2 p2 (Finished v m'')
+  -> exec_recover m p1 p2 (Crashed m'')
+| XRCrashCrash : forall R m p1 p2 m' m'', exec m p1 (@Crashed R m')
+  -> exec_recover m' p2 p2 (Crashed m'')
+  -> exec_recover m p1 p2 (Crashed m'').
 
 Hint Constructors exec.
 Hint Constructors exec_recover.
 
 
-Theorem exec_need_not_crash : forall p m,
-  exists m' out, exec m p m' out /\ out <> Crashed.
+Theorem exec_need_not_crash : forall R (p : prog R) m, exists out,
+  exec m p out /\ forall m', out <> Crashed m'.
 Proof.
-  induction p.
-  - do 2 eexists; split.
+  induction p; intros.
+  - eexists; split.
     constructor.
     discriminate.
-  - intros.
-    case_eq (m a); intros.
-    + edestruct H. destruct H1. destruct H1.
-      do 2 eexists; split.
-      * eapply XReadOK; eauto.
-      * auto.
-    + do 2 eexists; split.
-      * eapply XReadFail; eauto.
-      * discriminate.
-  - intros.
-    case_eq (m a); intros.
-    + edestruct H. destruct H1. destruct H1.
-      do 2 eexists; split.
-      * eapply XWriteOK; eauto.
-      * auto.
-    + do 2 eexists; split.
-      * eapply XWriteFail; eauto.
-      * discriminate.
+  - case_eq (m a); intros.
+    + eexists; split; [ eapply XReadOK; eauto | discriminate ].
+    + eexists; split; [ eapply XReadFail; eauto | discriminate ].
+  - case_eq (m a); intros.
+    + eexists; split; [ eapply XWriteOK; eauto | discriminate ].
+    + eexists; split; [ eapply XWriteFail; eauto | discriminate ].
+  - edestruct IHp; destruct x.
+    + eexists; split; [ eapply XSeqFail; intuition eauto | discriminate ].
+    + intuition congruence.
+    + edestruct H.
+      eexists; split; [ eapply XSeqOK; intuition eauto | intuition eauto ].
 Qed.
 
-Theorem exec_recover_can_terminate : forall p1 p2 m,
-  exists m' out, exec_recover m p1 p2 m' out.
+Theorem exec_recover_can_terminate : forall R (p1: prog R) p2 m,
+  exists out, exec_recover m p1 p2 out.
 Proof.
   intros.
   destruct (exec_need_not_crash p1 m).
-  destruct H. destruct H.
-  do 2 eexists.
-  destruct x0; try congruence.
-  - apply XRFail; eauto.
-  - apply XRFinished; eauto.
+  destruct x; ( try intuition congruence ) ; eexists.
+  - apply XRFail; intuition eauto.
+  - apply XRFinished; intuition eauto.
 Qed.
 
-Theorem prog_can_crash : forall p m m' out,
-  exec m p m' out ->
-  exec m p m' Crashed.
+Theorem prog_can_crash : forall R (p: prog R) m r m', exec m p (Finished r m') ->
+  exec m p (Crashed m').
 Proof.
-  induction p; intros.
-  - inversion H; eauto.
-  - inversion H0; eauto.
-  - inversion H0; eauto.
+  induction p; intros; try ( inversion H; eauto ).
+  inversion H0; eauto.
 Qed.
-
 
 Theorem upd_eq : forall m a v a',
   a' = a
